\begin{problem}
  Exercise 5.6 in Nocedal and Wright.

  Show that Eq.~(5.24d) 
  
  \[ \beta_{k+1} = \frac{r_{k+1}\transpose r_{k+1}}{r_{k}\transpose r_{k}} \]

  is equivalent to Eq.~(5.14d)

  \[ \beta_{k+1} = \frac{r_{k+1}\transpose Ap_{k}}{p_{k}\transpose Ap_{k}} \text{.}\]
\end{problem}


\noindent
Below is the extension of Eq.~(5.24d) to Eq.~(5.14d) using the equations and theorems in Nocedal and Wright.

\begin{proof}
  \begin{alignat*}{2}
    \beta_{k+1} &= \frac{r_{k+1}\transpose r_{k+1}}{r_{k}\transpose r_{k}} &\quad &\text{Nocedal \& Wright~(5.24d)} \\
    &= \frac{r_{k+1}\transpose r_{k+1}}{\alpha_{k}p\transpose_{k}Ap_{k}} &\quad &\text{Nocedal \& Wright~(5.24a)} \\
    &= \frac{r_{k+1}\transpose \left(r_{k} + \alpha_{k}p_{k}\right)}{\alpha_{k}p\transpose_{k}Ap_{k}} &\quad &\text{Nocedal \& Wright~(5.24c)} \\
    &= \frac{r_{k+1}\transpose \alpha_{k}Ap_{k}}{\alpha_{k}p\transpose_{k}Ap_{k}} &\quad &\text{Theorem~5.3 Eq.~(5.16)} \\
    &=\boxed{\frac{r\transpose_{k+1}Ap_{k}}{p\transpose_{k}Ap_{k}}} &\quad &\text{}
  \end{alignat*}
\end{proof}
%Eq.~(5.24a) specifies $\alpha_k$ as:
%
%\[\alpha_{k} = \frac{r\transpose_{k}r_{k}}{p\transpose_{k}Ap_{k}} \text{.} \]
%
%Substituting into Eq.~(5.24d), it equals:
%
%\[ \beta_{k+1} =  \]
%
%By Eq.~
